
### **Step One:**  
**1.** O(n + 10) = O(n)  
**2.** O(100 * n) = O(n)  
**3.** O(25) = O(1)  
**4.** O(n<sup>2</sup> + n<sup>3</sup>) = O(n<sup>3</sup>)  
**5.** O(n + n + n + n) = O(n)  
**6.** O(1000 * log(n) + n) = O(n)  
**7.** O(1000 * n * log(n) + n) = O(n * log(n))  
**8.** O(2<sup>n</sup> + n<sup>2</sup>) = O(2<sup>n</sup>)  
**9.** O(5 + 3 + 1) = O(1)  
**10.** O(n + n<sup>1/2</sup> + n<sup>2</sup> + n * log(n)<sup>10</sup>) = O(n<sup>2</sup>)  

### **Step Two:**
**1.** O(n)  
**2.** O(n)  
**3.** O(1)<sup>*</sup>  
**4.** O(n)  
**5.** O(n<sup>2</sup>)  
**6.** O(n)  

### **Step Three:**  
**1.** True  
**2.** True  
**3.** False  
**4.** O(n)  
**5.** O(n)  
**6.** O(n)  
**7.** O(n log n)<sup>#</sup>  
**8.** O(n)  
**9.** O(1)  
**10.** O(n)  
**11.** O(1)  
**12.** O(n)<sup>*</sup>  
**13.** O(n)  



















